wip

src/Init/Data/Iterators/Consumers/Monadic/Access.lean
@@ -8,6 +8,7 @@ module
 prelude
 public import Init.Data.Iterators.Basic
 public import Init.WFExtrinsicFix
+import Init.RCases
 
 set_option linter.missingDocs true
 
@@ -47,7 +48,7 @@ inductive IterM.IsPlausibleNthOutputStep {α β : Type w} {m : Type w → Type w
   | skip {it it' : IterM (α := α) m β} {step} : it.IsPlausibleStep (.skip it') →
       it'.IsPlausibleNthOutputStep n step → it.IsPlausibleNthOutputStep n step
 
-theorem IterM.not_isPlausibleNthOutputStep_yield {α β : Type w} {m : Type w → Type w'} [Iterator α m β]
+theorem IterM.not_isPlausibleNthOutputStep_skip {α β : Type w} {m : Type w → Type w'} [Iterator α m β]
     {n : Nat} {it it' : IterM (α := α) m β} :
     ¬ it.IsPlausibleNthOutputStep n (.skip it') := by
   intro h
@@ -57,6 +58,45 @@ theorem IterM.not_isPlausibleNthOutputStep_yield {α β : Type w} {m : Type w �
   · cases h'
   · simp_all
   · simp_all
+
+theorem IterM.isPlausibleNthOutputStep_trans_of_yield {α β : Type w} {m : Type w → Type w'}
+    [Iterator α m β] {k n} {it it' : IterM (α := α) m β} {out step}
+    (h : it.IsPlausibleNthOutputStep k (.yield it' out))
+    (h' : it'.IsPlausibleNthOutputStep n step) :
+    it.IsPlausibleNthOutputStep (n + k + 1) step := by
+  generalize hs : (IterStep.yield it' out) = s at h
+  induction h generalizing h' it' out
+  case zero_yield =>
+    cases hs
+    exact .yield ‹_› h'
+  case done => cases hs
+  case yield ih =>
+    cases hs
+    refine .yield ‹_› ?_
+    simp only [Nat.add_assoc] at ih
+    exact ih h' rfl
+  case skip ih =>
+    cases hs
+    refine .skip ‹_› ?_
+    apply ih h' rfl
+
+theorem IterM.isPlausibleNthOutputStep_trans_of_done {α β : Type w} {m : Type w → Type w'}
+    [Iterator α m β] {k n} {it : IterM (α := α) m β}
+    (h : it.IsPlausibleNthOutputStep k .done) (hle : k ≤ n) :
+    it.IsPlausibleNthOutputStep n .done := by
+  generalize hs : IterStep.done = s at h
+  induction h generalizing n
+  case zero_yield => cases hs
+  case yield ih =>
+    cases hs
+    obtain ⟨n, rfl⟩ := Nat.exists_eq_add_one_of_ne_zero (n := n) (Nat.ne_zero_of_lt (Nat.lt_of_add_one_le hle))
+    exact .yield ‹_› (ih (Nat.le_of_add_le_add_right hle) rfl)
+  case skip ih =>
+    cases hs
+    exact .skip ‹_› (ih hle rfl)
+  case done =>
+    cases hs
+    exact .done ‹_›
 
 /--
 `IteratorAccess α m` provides efficient implementations for random access or iterators that support
@@ -95,6 +135,28 @@ the `IteratorAccess` typeclass.
 def IterM.nextAtIdx? [Iterator α m β] [IteratorAccess α m] (it : IterM (α := α) m β)
     (n : Nat) : m (PlausibleIterStep (it.IsPlausibleNthOutputStep n)) :=
   IteratorAccess.nextAtIdx? it n
+
+/--
+Slow version of `IterM.nextAtIdx?` that does not require an `IteratorAccess α m` instance.
+
+Returns the step in which `it` yields its `n`-th element, or `.done` if it terminates earlier.
+In contrast to `step`, this function will always return either `.yield` or `.done` but never a
+`.skip` step.
+
+This function terminates after finitely many steps.
+-/
+@[inline]
+def IterM.atIdxSlow? [Monad m] [Iterator α m β] [Productive α m]
+    (it' : IterM (α := α) m β)
+    (n' : Nat) : m (Option β) := do
+    match (← it'.step).inflate with
+    | .yield it'' out _ =>
+      match n' with
+      | 0 => return some out
+      | k + 1 => atIdxSlow? it'' k
+    | .skip it'' _ => atIdxSlow? it'' n'
+    | .done _ => return none
+  termination_by (n', it'.finitelyManySkips)
 
 /--
 Slow version of `IterM.nextAtIdx?` that does not require an `IteratorAccess α m` instance.
