src/Std/Data/Iterators/Combinators/Monadic/StepSize.lean
@@ -59,7 +59,7 @@ def IterM.stepSize [Iterator α m β] [IteratorAccess α m] [Monad m]
 def IterM.Intermediate.stepSize [Iterator α m β] [IteratorAccess α m] [Monad m]
     (it : IterM (α := α) m β) (nextIdx : Nat) (n : Nat) :
     IterM (α := Types.StepSizeIterator α m β) m β :=
-  ⟨⟨0, nextIdx, it⟩⟩
+  ⟨⟨nextIdx, n - 1, it⟩⟩
 
 namespace Iterators.Types
 
