src/Init/Data/Iterators/Lemmas/Consumers/Access.lean
@@ -7,9 +7,34 @@ module
 
 prelude
 public import Init.Data.Iterators.Consumers.Access
+import Init.Data.Iterators.Lemmas.Consumers.Monadic.Access
 
 namespace Std.Iter
 open Std.Iterators
+
+public theorem nextAtIdxSlow?_eq_match [Iterator α Id β] [Productive α Id]
+    {n : Nat} {it : Iter (α := α) β} :
+    it.nextAtIdxSlow? n =
+      (match it.step with
+      | .yield it' out hp =>
+        match n with
+        | 0 => .yield it' out (.zero_yield hp)
+        | n + 1 =>
+          let s := it'.nextAtIdxSlow? n
+          ⟨s.val, .yield hp s.property⟩
+      | .skip it' hp =>
+        let s := it'.nextAtIdxSlow? n
+        ⟨s.val, .skip hp s.property⟩
+      | .done hp => .done (.done hp)) := by
+  simp [Iter.nextAtIdxSlow?]
+  apply Subtype.ext
+  simp only
+  rw [IterM.nextAtIdxSlow?_eq_match]
+  simp only [bind_pure_comp, Id.run_bind, step]
+  split
+  · cases n <;> simp [*]
+  · simp [*]
+  · simp [*]
 
 public theorem atIdxSlow?_eq_match [Iterator α Id β] [Productive α Id]
     {n : Nat} {it : Iter (α := α) β} :
