src/Init/Data/Iterators/Lemmas/Consumers/Monadic/Access.lean
@@ -1,0 +1,139 @@
+/-
+Copyright (c) 2026 Lean FRO, LLC. All rights reserved.
+Released under Apache 2.0 license as described in the file LICENSE.
+Authors: Paul Reichert
+-/
+module
+
+prelude
+public import Init.Data.Iterators.Consumers.Monadic.Access
+import all Init.Data.Iterators.Consumers.Monadic.Access
+public import Init.Control.Lawful.Basic
+import Init.Control.Lawful.Lemmas
+
+namespace Std.IterM
+open Std.Iterators
+
+
+public theorem atIdxSlow?_eq_match [Monad m] [LawfulMonad m] [Iterator α m β] [Productive α m]
+    {n : Nat} {it : IterM (α := α) m β} :
+    it.atIdxSlow? n = (do
+      match (← it.step).inflate.val with
+      | .yield it' out =>
+        match n with
+        | 0 => return some out
+        | n + 1 => it'.atIdxSlow? n
+      | .skip it' => it'.atIdxSlow? n
+      | .done => return none) := by
+  sorry
+
+private theorem val_nextAtIdxSlow?Go [Monad m] [LawfulMonad m] [Iterator α m β] [Productive α m]
+    {n : Nat} {it : IterM (α := α) m β} {n' it' h} :
+    Subtype.val <$> IterM.nextAtIdxSlow?.go it n it' n' h =
+      Subtype.val <$> IterM.nextAtIdxSlow? it' n' := by
+  induction it', n' using IterM.atIdxSlow?.induct generalizing it n
+  rw [IterM.nextAtIdxSlow?, IterM.nextAtIdxSlow?.go, IterM.nextAtIdxSlow?.go]
+  simp only [map_eq_pure_bind, bind_assoc]
+  apply bind_congr; intro step
+  rename_i it' n' ih₁ ih₂
+  cases step.inflate using PlausibleIterStep.casesOn
+  · simp
+    cases n'
+    · simp
+    · simp only at ih₁
+      simp [ih₁]
+  · simp only at ih₂
+    simp (discharger := assumption) [ih₂]
+  · simp
+
+public theorem val_nextAtIdxSlow?_eq_match [Monad m] [LawfulMonad m] [Iterator α m β] [Productive α m]
+    {n : Nat} {it : IterM (α := α) m β} :
+    Subtype.val <$> it.nextAtIdxSlow? n = (do
+      match (← it.step).inflate.val with
+      | .yield it' out =>
+        match n with
+        | 0 => return .yield it' out
+        | n + 1 => return (← it'.nextAtIdxSlow? n).val
+      | .skip it' => return (← it'.nextAtIdxSlow? n).val
+      | .done =>
+        return .done) := by
+  rw [IterM.nextAtIdxSlow?, IterM.nextAtIdxSlow?.go]
+  simp only [map_eq_pure_bind, bind_assoc]
+  apply bind_congr; intro step
+  cases step.inflate using PlausibleIterStep.casesOn
+  · cases n
+    · simp
+    · simp [val_nextAtIdxSlow?Go]
+  · simp [val_nextAtIdxSlow?Go]
+  · simp
+
+public theorem nextAtIdxSlow?_eq_match [Monad m] [LawfulMonad m] [Iterator α m β] [Productive α m]
+    {n : Nat} {it : IterM (α := α) m β} :
+    it.nextAtIdxSlow? n = (do
+      match (← it.step).inflate with
+      | .yield it' out hp =>
+        match n with
+        | 0 => return .yield it' out (.zero_yield hp)
+        | n + 1 =>
+          let s ← it'.nextAtIdxSlow? n
+          return ⟨s.val, .yield hp s.property⟩
+      | .skip it' hp =>
+          let s ← it'.nextAtIdxSlow? n
+          return ⟨s.val, .skip hp s.property⟩
+      | .done hp =>
+        return .done (.done hp)) := by
+  apply (map_inj_right Subtype.ext).mp
+  rw [val_nextAtIdxSlow?_eq_match]
+  simp only [map_eq_pure_bind, bind_assoc]
+  apply bind_congr; intro step
+  cases step.inflate using PlausibleIterStep.casesOn
+  · cases n <;> simp
+  · simp
+  · simp
+
+public theorem nextAtIdxSlow?_eq_match_nextAtIdxSlow? [Monad m] [LawfulMonad m] [Iterator α m β] [Productive α m]
+    {n : Nat} {it : IterM (α := α) m β} :
+    it.nextAtIdxSlow? n = (do
+      let step ← it.nextAtIdxSlow? 0
+      match n with
+      | 0 => return step
+      | n + 1 =>
+        match step with
+        | .yield it' out hp =>
+          let s ← it'.nextAtIdxSlow? n
+          return ⟨s.val, isPlausibleNthOutputStep_trans_of_yield hp s.property⟩
+        | .skip it' hp => not_isPlausibleNthOutputStep_skip.elim hp
+        | .done hp => return ⟨.done, isPlausibleNthOutputStep_trans_of_done (k := 0) hp (Nat.zero_le _)⟩) := by
+  fun_induction it.atIdxSlow? n
+  rename_i ih₁ ih₂
+  rw [nextAtIdxSlow?_eq_match, nextAtIdxSlow?_eq_match]
+  simp only [bind_assoc]
+  apply bind_congr; intro step
+  cases step.inflate using PlausibleIterStep.casesOn
+  · simp
+  · simp
+    simp at ih₁ ih₂
+    rw [ih₂]
+    · simp
+      apply bind_congr; intro step'
+      split
+      · simp
+      · simp
+        split
+        · simp
+        · exact not_isPlausibleNthOutputStep_skip.elim ‹_›
+        · simp
+    · assumption
+  · simp
+    split <;> simp
+
+public theorem nextAtIdxSlow?_add_one [Monad m] [LawfulMonad m] [Iterator α m β] [Productive α m]
+    {n : Nat} {it : IterM (α := α) m β} :
+    it.nextAtIdxSlow? (n + 1) = (do
+      match ← it.nextAtIdxSlow? 0 with
+      | .yield it' _ hp =>
+        let s ← it'.nextAtIdxSlow? n
+        return ⟨s.val, isPlausibleNthOutputStep_trans_of_yield hp s.property⟩
+      | .skip _ hp => not_isPlausibleNthOutputStep_skip.elim hp
+      | .done hp => return ⟨.done, isPlausibleNthOutputStep_trans_of_done (k := 0) hp (Nat.zero_le _)⟩) := by
+  rw [nextAtIdxSlow?_eq_match_nextAtIdxSlow?]
