src/Std/Data/Iterators/Lemmas/Combinators/StepSize.lean
@@ -8,9 +8,15 @@ module
 prelude
 public import Init.Data.Iterators.Consumers.Access
 public import Init.Data.Iterators.Consumers.Collect
+public import Init.Data.Iterators.Consumers.Loop
 public import Init.Data.Iterators.Combinators.Take
 public import Std.Data.Iterators.Combinators.StepSize
 import Init.Data.Iterators.Lemmas.Consumers.Access
+import Init.Data.Iterators.Lemmas.Consumers.Monadic.Access
+import Init.Data.Iterators.Lemmas.Consumers.Monadic.Loop
+import Init.Data.Iterators.Lemmas.Monadic.Basic
+import all Init.Data.Iterators.Consumers.Monadic.Access
+import all Std.Data.Iterators.Combinators.StepSize
 
 public section
 open Std Std.Iterators Std.Iterators.Types
@@ -125,16 +131,157 @@ instance [Iterator α Id β] [LawfulDeterministicIterator α Id] {it : IterM (α
     have := IterM.eq_of_isPlausibleNthOutputStep_of_isPlausibleNthOutputStep hs hs'
     rwa [Subtype.mk.injEq]
 
-theorem _root_.Std.IterM.step_stepSize [Iterator α Id β] [Productive α Id] [LawfulDeterministicIterator α Id]
+theorem _root_.Std.IterM.nextAtIdx?_eq_nextAtIdxSlow? [Iterator α Id β] [Productive α Id] [LawfulDeterministicIterator α Id]
     [IteratorAccess α Id] {it : IterM (α := α) Id β} {n : Nat} :
     it.nextAtIdx? n = it.nextAtIdxSlow? n := by
   ext
   apply Subsingleton.allEq
 
-theorem step_stepSize [Iterator α Id β] [Productive α Id] [LawfulDeterministicIterator α Id]
+theorem nextAtIdx?_eq_nextAtIdxSlow? [Iterator α Id β] [Productive α Id] [LawfulDeterministicIterator α Id]
     [IteratorAccess α Id] {it : Iter (α := α) β} {n : Nat} :
     it.nextAtIdx? n = it.nextAtIdxSlow? n := by
-  simp [Iter.nextAtIdx?, Iter.nextAtIdxSlow?, IterM.step_stepSize]
+  simp [Iter.nextAtIdx?, Iter.nextAtIdxSlow?, IterM.nextAtIdx?_eq_nextAtIdxSlow?]
+
+theorem _root_.Std.IterM.nextAtIdxSlow?_stepSize_aux [Iterator α Id β] [Productive α Id] [LawfulDeterministicIterator α Id]
+    [IteratorAccess α Id] {it : IterM (α := α) Id β} {n : Nat} :
+    (IterM.Intermediate.stepSize it i n).nextAtIdxSlow? 0 = (do
+      match (← it.nextAtIdxSlow? i) with
+      | .yield it' out h =>
+        return .yield (IterM.Intermediate.stepSize it' (n - 1) n) out (by
+          refine .zero_yield ?_
+          simpa [IterM.IsPlausibleStep, Iterator.IsPlausibleStep,
+            IterM.Intermediate.stepSize, IterM.Intermediate.stepSize])
+      | .skip it' h => return IterM.not_isPlausibleNthOutputStep_skip.elim h
+      | .done h =>
+        return .done (by
+          refine .done ?_
+          simpa [IterM.IsPlausibleStep, Iterator.IsPlausibleStep,
+            Intermediate.stepSize, IterM.Intermediate.stepSize])) := by
+  induction it, i using IterM.atIdxSlow?.induct_unfolding
+  simp [IterM.Intermediate.stepSize]
+  rw [IterM.nextAtIdxSlow?_eq_match]
+  simp [IterM.step_eq, IterM.nextAtIdx?_eq_nextAtIdxSlow?]
+  apply bind_congr; intro step
+  cases step using PlausibleIterStep.casesOn
+  · simp
+  · exact IterM.not_isPlausibleNthOutputStep_skip.elim ‹_›
+  · simp
+
+theorem _root_.Std.IterM.length_nextAtIdxSlow? [Monad m] [LawfulMonad m] [Iterator α m β] [Finite α m] [IteratorLoop α m m] [LawfulIteratorLoop α m m]
+    {it : IterM (α := α) m β} :
+    (do match ← it.nextAtIdxSlow? n with
+      | .yield it' out _ => it'.length
+      | .skip it' h => IterM.not_isPlausibleNthOutputStep_skip.elim h
+      | .done h => return .up 0) = (fun len => .up (len.down - n - 1)) <$> it.length := by
+  induction it using IterM.inductSteps generalizing n with | step it ihy ihs
+  rw [it.nextAtIdxSlow?_eq_match, it.length_eq_match_step]
+  simp only [map_eq_pure_bind, bind_assoc]
+  apply bind_congr; intro step
+  cases step.inflate using PlausibleIterStep.casesOn
+  · simp
+    split
+    · simp
+    · rename_i it' out h n n'
+      simp
+      refine Eq.trans ?_ ((ihy h (n := n')).trans ?_)
+      · apply bind_congr; intro step
+        cases step using PlausibleIterStep.casesOn
+        · simp
+        · rfl
+        · simp
+      · simp [Nat.add_sub_add_right]
+  · rename_i it' h n _ h
+    simp
+    refine Eq.trans ?_ ((ihs h (n := n)).trans ?_)
+    · apply bind_congr; intro step
+      cases step using PlausibleIterStep.casesOn
+      · simp
+      · rfl
+      · simp
+    · simp
+  · simp
+
+theorem length_nextAtIdxSlow? [Iterator α Id β] [Finite α Id] [IteratorLoop α Id Id] [LawfulIteratorLoop α Id Id]
+    {it : Iter (α := α) β} :
+    (match it.nextAtIdxSlow? n with
+      | .yield it' out _ => it'.length
+      | .skip it' h => IterM.not_isPlausibleNthOutputStep_skip.elim h
+      | .done h => 0) = it.length - n - 1 := by
+  have := IterM.length_nextAtIdxSlow? (it := it.toIterM) (n := n)
+  replace this := congrArg Id.run this
+  replace this := congrArg ULift.down this
+  simp at this
+  simp [Iter.length, ← this, Iter.nextAtIdxSlow?]
+  split at this
+  · simp [*]
+  · exact IterM.not_isPlausibleNthOutputStep_skip.elim ‹_›
+  · simp [*]
+
+theorem _root_.Std.IterM.length_stepSize [Iterator α Id β] [Finite α Id] [IteratorLoop α Id Id] [LawfulIteratorLoop α Id Id]
+    [IteratorAccess α Id] {it : IterM (α := α) Id β} :
+    (IterM.Intermediate.stepSize it i n).length.run.down = (it.length.run.down + (n - 1) - i) / (n - 1 + 1) := by
+  induction n generalizing it i
+  · rw [IterM.length_eq_match_step, IterM.length_eq_match_step, IterM.step_eq]
+    simp [IterM.Intermediate.stepSize]
+    cases (it.nextAtIdx? i).run using PlausibleIterStep.casesOn
+    · simp
+      rw [IterM.length_eq_match_step]
+      simp
+
+theorem _root_.Std.IterM.step_stepSize [Iterator α Id β] [Finite α Id] [LawfulDeterministicIterator α Id]
+    [IteratorAccess α Id] {it : IterM (α := α) Id β} :
+    (IterM.Intermediate.stepSize it i n).step.run.inflate.val =
+      match it.step.run.inflate.val with
+      | .yield it' out =>
+        match i with
+        | 0 => .yield (IterM.Intermediate.stepSize it' (n - 1) n) out
+        | i + 1 => .skip (IterM.Intermediate.stepSize it' i n)
+      | .skip it' => .skip (IterM.Intermediate.stepSize it' i n)
+      | .done => .done := by
+  rw [IterM.step_eq]
+  simp [IterM.Intermediate.stepSize, IterM.nextAtIdx?_eq_nextAtIdxSlow?]
+  rw [IterM.nextAtIdxSlow?_eq_match]
+  simp
+  cases it.step.run.inflate using PlausibleIterStep.casesOn
+  · simp
+    split
+    · simp
+    · simp
+
+
+theorem _root_.Std.IterM.length_stepSize [Iterator α Id β] [Finite α Id] [LawfulDeterministicIterator α Id]
+    [IteratorAccess α Id] [IteratorLoop α Id Id] [LawfulIteratorLoop α Id Id] {it : IterM (α := α) Id β} {i n : Nat} :
+    (IterM.Intermediate.stepSize it i n).length.run.down = (it.length.run.down + (n - 1) - i) / (n - 1 + 1) := by
+  induction it using IterM.inductSteps with | step it ihy ihs
+  rw [IterM.length_eq_match_step, IterM.length_eq_match_step, step_stepSize]
+
+theorem atIdxSlow?_stepSize_aux [Iterator α Id β] [Productive α Id] [LawfulDeterministicIterator α Id]
+    [IteratorAccess α Id] {it : Iter (α := α) β} {n : Nat} :
+    (Intermediate.stepSize it i n).nextAtIdxSlow? 0 =
+      match it.nextAtIdxSlow? i with
+      | .yield it' out h =>
+        .yield (Intermediate.stepSize it' (n - 1) n) out (by
+          refine .zero_yield ?_
+          simpa [IterM.IsPlausibleStep, Iterator.IsPlausibleStep,
+            Intermediate.stepSize, IterM.Intermediate.stepSize])
+      | .skip it' h => IterM.not_isPlausibleNthOutputStep_skip.elim h
+      | .done h =>
+        .done (by
+          refine .done ?_
+          simpa [IterM.IsPlausibleStep, Iterator.IsPlausibleStep,
+            Intermediate.stepSize, IterM.Intermediate.stepSize]) := by
+  simp only [Iter.nextAtIdxSlow?]
+  simp only [Intermediate.stepSize, toIterM_toIter, IterM.nextAtIdxSlow?_stepSize_aux]
+  simp
+  apply Subtype.ext
+  simp
+  let step := (it.toIterM.nextAtIdxSlow? i).run
+  cases hs : step using PlausibleIterStep.casesOn
+  · simp [show (it.toIterM.nextAtIdxSlow? i).run = step from rfl]
+    simp [hs]
+  · exact IterM.not_isPlausibleNthOutputStep_skip.elim ‹_›
+  · simp [show (it.toIterM.nextAtIdxSlow? i).run = step from rfl]
+    simp [hs]
 
 theorem atIdxSlow?_stepSize_aux [Iterator α Id β] [Productive α Id] [LawfulDeterministicIterator α Id]
     [IteratorAccess α Id] {it : Iter (α := α) β} {n : Nat} :
@@ -161,6 +308,7 @@ theorem atIdxSlow?_stepSize_aux [Iterator α Id β] [Productive α Id] [LawfulDe
         cases IterM.eq_of_isPlausibleNthOutputStep_of_isPlausibleNthOutputStep h h'
     case yield_succ it it' _ h _ =>
       rw [atIdxSlow?_eq_match, atIdxSlow?_eq_match]
+
   generalize h : Iter.Intermediate.stepSize it i n = sit
   induction k, sit using Iter.atIdxSlow?.induct_unfolding
   case yield_zero =>
